\documentclass[12pt]{amsart}

\usepackage{a4wide, amsxtra}

\usepackage[pdftex]{graphicx}

 \title{PMTH212 Assignment 3}

 \author{Mark Villar}

\begin{document} 

\maketitle 

\begin{enumerate}
	
	\item
		\begin{align*}
			&x(t)=e^t\cos t, \ \ \ \ y(t)=e^t\sin t, \ \ \ \ z(t)=e^t, \ \ \ \ t=0 \\
			&x'(t)=e^t\cos t-e^t\sin t=e^t(\cos t-\sin t) \ \Rightarrow \ x'(0)=1 \\
			&y'(t)=e^t\sin t+e^t\cos t=e^t(\cos t+\sin t) \ \Rightarrow \ y'(0)=1 \\ 
			&z'(t)=e^t \ \Rightarrow \ z'(0)=1 \\
			&||\mathbf{r}'(t)||=\sqrt{e^{2t}(1-2\sin t\cos t)+e^{2t}(1+2\sin t\cos t)+e^{2t}} \\
			&\ \ \ \ \ \ \ \ \ =\sqrt{e^{2t}+e^{2t}+e^{2t}}=\sqrt{3e^{2t}}=\sqrt{3}e^t \\
			&||\mathbf{r}'(0)||=\sqrt{1^2+1^2+1^2}=\sqrt{3}e^0=\sqrt{3} \\
			&\mathbf{T}(t)=\frac{\cos t-\sin t}{\sqrt{3}}\mathbf{i}+\frac{\cos t+\sin t}{\sqrt{3}}\mathbf{j}+\frac{1}
			{\sqrt{3}}\mathbf{k} \\
			&\mathbf{T}(0)=\frac{\mathbf{r}'(0)}{||\mathbf{r}'(0)||}=\frac{1}{\sqrt{3}}\mathbf{i}+\frac{1}{\sqrt{3}}			\mathbf{j}+\frac{1}{\sqrt{3}}\mathbf{k} \\
			&\mathbf{T}'(t)=\frac{-\sin t-\cos t}{\sqrt{3}}\mathbf{i}+\frac{-\sin t+\cos t}{\sqrt{3}}\mathbf{j}+0				\mathbf{k} \\
			&\ \ \ \ \ \ \ =-\frac{\cos t+\sin t}{\sqrt{3}}\mathbf{i}+\frac{\cos t-\sin t}{\sqrt{3}}\mathbf{j} \\
			&\mathbf{T}'(0)=-\frac{1}{\sqrt{3}}\mathbf{i}+\frac{1}{\sqrt{3}}\mathbf{j} \\
			&||\mathbf{T}'(t)||=\sqrt{\frac{1+2\sin t \cos t}{3}+\frac{1-2\sin t \cos t}{3}}=\sqrt{\frac{2}{3}} \\
			&\mathbf{N}(0)=\frac{\mathbf{T}'(0)}{||\mathbf{T}'(0)||}=-\frac{1}{\sqrt{2}}\mathbf{i}+\frac{1}{\sqrt{2}}			\mathbf{j}
		\end{align*}
		
	\item
		\begin{align*}	
			&\mathbf{r}(t)=e^t\mathbf{i}+e^{-t}\mathbf{j}+t\mathbf{k} \\
			&\mathbf{r}'(t)=e^t\mathbf{i}-e^{-t}\mathbf{j}+\mathbf{k} \\
			&\mathbf{r}''(t)=e^t\mathbf{i}+e^{-t}\mathbf{j}
		\end{align*}
		\begin{align*}
			\mathbf{r}'(t)\times\mathbf{r}''(t)=
				\begin{vmatrix}
					&\mathbf{i} \ &\ \mathbf{j} \ &\mathbf{k} \ \ \\
					&e^t \ &-e^{-t} \ &1 \ \ \\
					&e^t \ &\ \ e^{-t} \ &0 \ \ \\
				\end{vmatrix} 
			&=(0-e^{-t})\mathbf{i}-(0-e^t)\mathbf{j}+(1+1)\mathbf{k} \\
			&=-e^{-t}\mathbf{i}+e^t\mathbf{j}+2\mathbf{k}
		\end{align*}
		\begin{align*}
			&||\mathbf{r}'(t)||=\sqrt{e^{2t}+e^{-2t}+1^2} =\sqrt{1+1+1}=\sqrt{3} \ \text{ for } \ t=0 \\
			&||\mathbf{r}'(t)\times\mathbf{r}''(t)||=\sqrt{e^{-2t}+e^{2t}+2^2}=\sqrt{1+1+4}=\sqrt{6} \ \text{ for } \ 			t=0 \\
			&\kappa(0)=\frac{\sqrt{6}}{(\sqrt{3})^3}=\frac{\sqrt{6}}{3\sqrt{3}}=\frac{\sqrt{2}}{3} \\
		\end{align*}	
		
	\item We assume that $\mathbf{r}(x)$ is smooth and show that $\mathbf{r}''(x)$ and $\mathbf{T}'(x)$ exist.
		\begin{align*}
			&\mathbf{r}(x)=x\mathbf{i}+y\mathbf{j}=x\mathbf{i}+f(x)\mathbf{j} \\
			&\mathbf{r}'(x)=\mathbf{i}+\frac{dy}{dx}\mathbf{j} \ \Rightarrow \ \mathbf{r}''(x)=\frac{d^2y}{dx^2}\mathbf{j} \\
			&||\mathbf{r}'(x)||=\sqrt{1^2+\left(\frac{dy}{dx}\right)^2}=\left[1+\left(\frac{dy}{dx}\right)^2\right]^{\frac{1}{2}} \\
			&\mathbf{T}(x)=\frac{1}{\sqrt{1+\left(\frac{dy}{dx}\right)^2}}\mathbf{i}+\frac{dy}{dx}\frac{1}{\sqrt{1+\left(\frac{dy}{dx}\right)^2}}\mathbf{j} \\		
			&\mathbf{T}'(x)=-\frac{\frac{dy}{dx}\frac{d^2y}{dx^2}}{\left[1+\left(\frac{dy}{dx}\right)^2\right]^{\frac{3}{2}}}\mathbf{i} 		
			+\frac{\frac{d^2y}{dx^2}}{\left[1+\left(\frac{dy}{dx}\right)^2\right]^{\frac{3}{2}}}\mathbf{j}
		\end{align*}
		Hence,
			\begin{align*}
				&\kappa(x)=\frac{||\mathbf{r}'(x)\times \mathbf{r}''(x)||}{||\mathbf{r}'(x)||^3} \\
				&\mathbf{r}'(x)\times \mathbf{r}''(x)=
					\begin{vmatrix}
						&\mathbf{i} \ &\ \mathbf{j} \ &\mathbf{k} \ \ \\
						&1 \ &\frac{dy}{dx} \ &0 \ \ \\
						&0 \ &\ \frac{d^2y}{dx^2} \ &0 \ \ \\
					\end{vmatrix} 
					=0\mathbf{i}-0\mathbf{j}+\frac{d^2y}{dx^2}\mathbf{k} \\
					&||\mathbf{r}'(x)\times \mathbf{r}''(x)||=\sqrt{\left(\frac{d^2y}{dx^2}\right)^2}=\left|\frac{d^2y}{dx^2}\right| \\													
					&\kappa(x)=\frac{\left|\frac{d^2y}{dx^2}\right|}{\left[\left(1+\left(\frac{dy}{dx}\right)^2\right)^{\frac{1}{2}}\right]^3}=\frac{\left|\frac{d^2y}{dx^2}\right|}  
					{\left[1+\left(\frac{dy}{dx}\right)^2\right]^{\frac{3}{2}}} \\
			\end{align*}
			
	\item $f(x,y)=x+(xy)^{\frac{1}{3}}$
		\begin{enumerate}
			\item $f(t,t^2)=t+(t\cdot t^2)^{\frac{1}{3}}=t+t=2t$
			\item $f(x,x^2)=t+(x\cdot x^2)^{\frac{1}{3}}=x+x=2x$
			\item $f(2y^2,4y)=2y^2+(2y^2\cdot 4y)^{\frac{1}{3}}=2y^2+(8y^3)^{\frac{1}{3}}=2y^2+2y=2y(y+1)$ \\
		\end{enumerate}
	
	\item $g(u(x,y),v(x,y))=\pi xy\sin(x^4y^6\pi xy)=\pi xy\sin(\pi x^5y^7)$ \\
					
	\item $f(x,y,z)=zxy+x$
		\begin{enumerate}
			\item $f(x+y,x-y,x^2)=x^2(x+y)(x-y)+(x+y)=x^2(x^2-y^2)+x+y$				
			\item $f(xy,y/x, xz)=xz\cdot xy\cdot \dfrac{y}{x}+xy=xy^2z+xy=xy(yz+1)$ \\
		\end{enumerate}
		
	\item
		\begin{enumerate}
			\item $f(x,y,z)=3x-y+2z=k$
				\begin{align*}
					\bold{k=0:} \ &3x-y+2z=0 \ \text{is a plane with the following three points} \\
					&(0,0,0), (1,1,-1), (-1,-1,1) \ \text{lying on the plane.} \\
					\bold{k=1:} \ &3x-y+2z=1 \ \text{is a plane parallel to} \ 3x-y+2z=0 \\
					&\text{which intersects the} \ z\text{-axis at} \ (0,0,1/2).
				\end{align*}	
				\begin{align*}
					&\ \ \ \ \ \text{For any} \ k, \ \text{the level surface is the plane} \ 3x-y+2z=k, \ \text{parallel to} \\
					&\ \ \ \ \ 3x-y+2z=0 \ \text{which intersects the} \ z\text{-axis at} \ (0,0,k/2).
				\end{align*}					
			\item $f(x,y,z)=z-x^2-y^2=k$
				\begin{align*}
					&\ \ \ \ \bold{k=0:} \ z=x^2+y^2 \ \text{is an elliptic paraboloid with centre} \ (0,0,0). \\
					&\ \ \ \ \bold{k=1:} \ z-1=x^2+y^2 \ \text{is an elliptic paraboloid with centre} \ (0,0,1).
				\end{align*}	
				\begin{align*}
					\ \ \ \ \ \ \ \ \ \ \text{For any} \ k, \ \text{the level surface is an elliptic paraboloid with centre} \ (0,0,k).
				\end{align*}			
		\end{enumerate}
		
\end{enumerate}

\end{document}
